UDP Packet Decoder Derivation done.

src/BinEncoders/Env/Examples/UDP_Packet.v
@@ -36,7 +36,7 @@ Open Scope Tuple_scope.
 
 Definition UDP_Packet :=
   @Tuple <"SourcePort" :: word 16,
-          "DestPort" :: word 16, (* Don't fragment flag *)
+          "DestPort" :: word 16,
           "Payload" :: list char >.
 
 Definition transformer : Transformer ByteString := ByteStringTransformer.
@@ -65,9 +65,7 @@ Definition encode_UDP_Packet_Spec
     ThenC encode_word_Spec (udp!"DestPort")
     ThenC encode_nat_Spec 16 (8 + |udp!"Payload"|) DoneC)
     ThenChecksum (UDP_Checksum_Valid srcAddr destAddr udpLength) OfSize 16
-    ThenCarryOn (encode_list_Spec encode_word_Spec udp!"Payload"
-             ThenC (if (Peano_dec.eq_nat_dec (NPeano.modulo (length udp!"Payload") 2) 0) then encode_word_Spec WO else encode_word_Spec (wzero 8))
-                                  DoneC).
+    ThenCarryOn (encode_list_Spec encode_word_Spec udp!"Payload" DoneC).
 
 Definition UDP_Packet_OK (udp : UDP_Packet) :=
   lt (|udp!"Payload"|) (pow2 16 - 8).
@@ -81,7 +79,7 @@ Definition UDP_Packet_encoded_measure (udp_b : ByteString)
   | None => 0
   end.
 
-Lemma if_computes_to_len {P}
+(*Lemma if_computes_to_len {P}
   : forall (b : {P} + {~P}) b' encodeT encodeE n n' ctx ctx',
     (forall b ctx ctx', encodeT ctx ↝ (b, ctx') -> length_ByteString b = n)
     -> (forall b (ctx ctx' : CacheEncode), encodeE ctx ↝ (b, ctx') -> length_ByteString b = n')
@@ -89,34 +87,51 @@ Lemma if_computes_to_len {P}
     -> length_ByteString b' = if b then n else n'.
 Proof.
   intros; find_if_inside; eauto.
-Qed.
+Qed. *)
 
 Arguments NPeano.modulo : simpl never.
 
-Lemma mod_16_even_8 :
-  forall n,
-    NPeano.modulo n 2 = 0
-    -> NPeano.modulo (n * 8 + 0) 16 = 0.
+Lemma lt_minus_plus :
+  forall n m o,
+    lt n (o - m) -> lt (m + n) o.
 Proof.
-  intros; rewrite <- plus_n_O.
-  rewrite Mult.mult_comm.
-  pose proof (NPeano.Nat.mul_mod_distr_l n 2 8).
-  unfold mult at 2 in H0; simpl in H0.
-  rewrite H0, H; eauto.
+  intros; omega.
 Qed.
 
-Lemma mod_16_odd_8 :
-  forall n,
-    NPeano.modulo n 2 <> 0
-    -> NPeano.modulo (n * 8) 16 = 8.
+Lemma mult_8_mod_8 :
+  forall n, NPeano.modulo (n * 8) 8 = 0.
 Proof.
-  intros; rewrite Mult.mult_comm.
-  pose proof (NPeano.Nat.mul_mod_distr_l n 2 8).
-  unfold mult at 2 in H0; simpl in H0.
-  rewrite H0; eauto.
-  pose proof (NPeano.Nat.mod_upper_bound n 2).
-  omega.
+  intros; eapply NPeano.Nat.mod_mul; eauto.
 Qed.
+
+Lemma lt_minus_minus :
+  forall n' n m o,
+    lt m o
+    -> n' = n - m
+    -> lt n o -> lt n' (o - m).
+Proof.
+  intros; omega.
+Qed.
+
+Lemma lt_8_2_16 : lt 8 (pow2 16).
+Proof.
+  rewrite <- Npow2_nat.
+  rewrite Compare_dec.nat_compare_lt.
+  rewrite <- (Nnat.Nat2N.id 8) at 1.
+  rewrite <- Nnat.N2Nat.inj_compare.
+  reflexivity.
+Qed.
+
+Lemma lt_minus_plus_idem :
+  forall n m o,
+    lt m o
+    -> lt n o
+    -> lt (m + (n - m)) o.
+Proof.
+  intros; omega.
+Qed.
+
+Opaque pow2.
 
 Definition UDP_Packet_decoder'
   : { decodePlusCacheInv |
@@ -153,15 +168,9 @@ Proof.
   reflexivity.
   repeat calculate_length_ByteString.
   repeat calculate_length_ByteString.
-  intros. eapply if_computes_to_len; eauto;
-            repeat calculate_length_ByteString.
-  solve_mod_16.
-  intros; cbv beta; find_if_inside.
-  solve_mod_16.
-  simpl; rewrite mod_16_even_8; eauto.
-  solve_mod_16; simpl.
-  intros; rewrite <- NPeano.Nat.add_mod_idemp_l; eauto.
-  simpl; rewrite mod_16_odd_8; eauto.
+  solve_mod_8.
+  solve_mod_8.
+  rewrite <- plus_n_O, mult_8_mod_8; eauto.
   { (* Grossest Proof By Far. *)
     intros; simpl transform_id; rewrite length_ByteString_ByteString_id.
     instantiate (1 := UDP_Packet_encoded_measure).
@@ -180,7 +189,6 @@ Proof.
       let H' := fresh in
       destruct H0 as [? [? [? H'] ] ]; rewrite H'.
     unfold fst.
-    find_if_inside.
     rewrite wordToNat_natToWord_idempotent; try reflexivity.
     rewrite !Plus.plus_assoc.
     clear.
@@ -202,8 +210,9 @@ Proof.
     rewrite <- BinNat.N.compare_lt_iff.
     rewrite Nnat.N2Nat.inj_compare.
     rewrite Nnat.Nat2N.id.
-    admit.
-    clear; admit.
+    rewrite <- Compare_dec.nat_compare_lt.
+    rewrite Npow2_nat.
+    omega.
   }
   apply_compose.
   eapply Word_decode_correct.
@@ -223,11 +232,16 @@ Proof.
     (1 := fun p b env => if Compare_dec.le_lt_dec p (pow2 16) then
                            _ p b env else None).
   simpl in *.
+  instantiate
+    (1 := fun p b env => if Compare_dec.lt_dec p 8 then
+                           None else _ p b env).
+  simpl in *.
   assert (b0 = proj1 - 8) by
       (rewrite <- H9; simpl; auto with arith).
   destruct (Compare_dec.le_lt_dec proj1 (pow2 16)).
-  rewrite H8; clear H8.
-  clear H9.
+  destruct (Compare_dec.lt_dec proj1 8).
+  elimtype False; omega.
+  rewrite H8; clear H8; clear H9.
   computes_to_inv; injections; subst; simpl.
   eexists env'; simpl; intuition eauto.
   rewrite ByteString_transform_id_left.
@@ -239,7 +253,7 @@ Proof.
   end.
   omega.
   simpl in H6.
-  find_if_inside; try discriminate.
+  repeat find_if_inside; try discriminate.
   simpl in H6; injections; eauto.
   simpl.
   eexists _; eexists tt;
@@ -250,19 +264,17 @@ Proof.
           end.
   destruct env; computes_to_econstructor.
   pose proof transform_id_left as H'; simpl in H'; rewrite H'.
-  find_if_inside; simpl in *; try discriminate;
+  repeat find_if_inside; simpl in *; try discriminate;
     injections.
   reflexivity.
   instantiate (1 := fun _ => True); eauto.
-  find_if_inside; try discriminate; injections.
-  clear; admit.
-  find_if_inside; try discriminate; injections; eauto.
-  find_if_inside; try discriminate; injections; eauto.
-  find_if_inside; try discriminate; injections; eauto.
-  clear; admit.
+  repeat find_if_inside; try discriminate; injections; eauto.
+  eapply (lt_minus_plus_idem _ 8); eauto using lt_8_2_16.
+  repeat find_if_inside; try discriminate; injections; eauto.
+  repeat find_if_inside; try discriminate; injections; eauto.
+  repeat find_if_inside; try discriminate; injections; eauto; omega.
   unfold UDP_Packet_OK; clear; intros ? H'; repeat split.
-  simpl.
-  clear; admit.
+  simpl; eapply lt_minus_plus with (m := 8); eauto.
   instantiate (1 := fun _ _ => True);
     simpl; intros; exact I.
   apply_compose.
@@ -270,77 +282,48 @@ Proof.
   eapply Word_decode_correct.
   eapply H'.
   simpl; intros; instantiate (1 := snd (snd proj)).
-  intuition.
-  destruct proj as [? [? ?] ]; simpl; injections; eauto.
+  intuition; subst; simpl; auto with arith.
+  destruct proj as [? [? ?] ]; simpl; injections.
   simpl; intros; eauto using FixedList_predicate_rest_True.
   intros.
-
-  eapply Word_decode_correct.
-  solve_data_inv.
-  solve_data_inv.
-  apply_compose.
-  intro; eapply FixList_decode_correct.
-  revert H3; eapply Word_decode_correct.
-  simpl in *; split.
-  intuition eauto.
-  eapply (f_equal fst H8).
-  intros; eauto.
-  simpl; intros; eauto using FixedList_predicate_rest_True.
-  simpl; intros;
-    unfold encode_decode_correct_f; intuition eauto.
-  destruct data as [? [? [? [? [? [? [? [? [? [? [ ] ] ] ] ] ] ] ] ] ] ];
+  unfold encode_decode_correct_f; intuition eauto.
+  destruct data as [? [? [? [ ] ] ] ];
     unfold GetAttribute, GetAttributeRaw in *;
     simpl in *.
-  pose proof (f_equal fst H14).
-  pose proof (f_equal (fun z => fst (snd z)) H14).
-  pose proof (f_equal (fun z => fst (snd (snd z))) H14).
-  pose proof (f_equal (fun z => fst (snd (snd (snd z)))) H14).
-  pose proof (f_equal (fun z => fst (snd (snd (snd (snd z))))) H14).
-  pose proof (f_equal (fun z => fst (snd (snd (snd (snd (snd z)))))) H14).
-  pose proof (f_equal (fun z => fst (snd (snd (snd (snd (snd (snd z))))))) H14).
-  pose proof (f_equal (fun z => fst (snd (snd (snd (snd (snd (snd z))))))) H14).
-  pose proof (f_equal (fun z => snd (snd (snd (snd (snd (snd (snd z))))))) H14).
+  pose proof (f_equal fst H9).
+  pose proof (f_equal (fun z => fst (snd z)) H9).
+  pose proof (f_equal (fun z => snd (snd z)) H9).
   simpl in *.
-  clear H14.
+  clear H9.
   computes_to_inv; injections; subst; simpl.
   pose proof transform_id_left as H'; simpl in H'; rewrite H'.
   eexists env'; simpl; intuition eauto.
   simpl in *.
-  simpl in H8; injections; eauto.
-  simpl in H8; repeat find_if_inside; try discriminate.
+  simpl in H5; injections; eauto.
+  simpl in H5; repeat find_if_inside; try discriminate.
   eexists _; eexists tt.
   injections; simpl in *; repeat split.
   destruct env; computes_to_econstructor.
   pose proof transform_id_left as H'; simpl in H'; rewrite H'.
   reflexivity.
+  unfold UDP_Packet_OK.
   unfold GetAttribute, GetAttributeRaw; simpl.
-  rewrite H5; eauto.
-  intuition.
+  split_and.
   simpl in *.
-  unfold pow2 in H9; simpl in H9; auto with arith.
-  omega.
-  unfold GetAttribute, GetAttributeRaw.
-  simpl.
-  rewrite H5.
-  omega.
-  destruct proj as [? [? [? [? [? [? [? ?] ] ] ] ] ] ].
-  simpl.
-  unfold GetAttribute, GetAttributeRaw; simpl in *.
-  repeat f_equal.
-  eauto.
-  simpl.
+  eapply lt_minus_minus; eauto using lt_8_2_16.
+  rewrite <- H5; simpl; rewrite <- Minus.minus_n_O; reflexivity.
+  destruct proj as [? [? ? ] ];
+    unfold GetAttribute, GetAttributeRaw in *;
+    simpl in *.
+  split_and; repeat f_equal; eauto.
   repeat (instantiate (1 := fun _ => True)).
   unfold cache_inv_Property; intuition.
-  Grab Existential Variables.
-  decide equality.
-  decide equality.
-  exact (@weq _).
 Defined.
 
-Definition IPv4_decoder_impl :=
-  Eval simpl in (fst (projT1 EthernetHeader_decoder)).
+Definition UDP_Packet_decoder_impl :=
+  Eval simpl in (fst (projT1 UDP_Packet_decoder')).
 
-Print IPv4_decoder_impl.
+Print UDP_Packet_decoder_impl.
 
 
 Lemma UDP_Packet_Headiner_Len_Bound
