src/BinEncoders/Env/Examples/EthernetHeader.v
@@ -37,7 +37,7 @@ Ltac apply_compose :=
   intros;
   match goal with
     H : cache_inv_Property ?P ?P_inv |- _ =>
-    first [eapply (compose_encode_correct_no_dep H); clear H
+    first [eapply (compose_encode_correct_no_dep _ H); clear H
           | eapply (compose_encode_correct H); clear H
           | eapply (composeIf_encode_correct H); clear H;
             [ |
