src/BinEncoders/Env/Examples/IPv4Header.v
@@ -169,8 +169,8 @@ Proof.
                                    DoneC))).
   repeat calculate_length_ByteString.
   repeat calculate_length_ByteString.
-  solve_mod_16.
-  solve_mod_16.
+  solve_mod_8.
+  solve_mod_8.
   { (* Grossest Proof By Far. *)
     intros; simpl transform_id; rewrite length_ByteString_ByteString_id.
     instantiate (1 := IPv4_Packet_encoded_measure).
